$\frac{2^n+3^n}{3 \cdot 2^{n+1}+2 \cdot 3^{n-1}}=\frac{2^n+3^n}{6 \cdot 2^n+\frac{2}{3} \cdot 3^n}=\frac{3^n\left(\left(\frac{2}{3}\right)^n+1\right)}{3^n\left(6 \cdot\left(\frac{2}{3}\right)^n+\frac{2}{3}\right)}=\frac{\left(\frac{2}{3}\right)^n+1}{6 \cdot\left(\frac{2}{3}\right)^n+\frac{2}{3}}$

$\lim _{n \rightarrow \infty} \frac{2^n+3^n}{3 \cdot 2^{n+1}+2 \cdot 3^{n-1}}=\lim _{n \rightarrow \infty} \frac{\left(\frac{2}{3}\right)^n+1}{6 \cdot\left(\frac{2}{3}\right)^n+\frac{2}{3}}=\frac{0+1}{6 \cdot 0+\frac{2}{3}}=\frac{1}{\frac{2}{3}}=\frac{3}{2}$

$Given\ x>1\qquad
\begin{aligned} \frac{\sqrt{x}}{\sqrt{x+\sqrt{x}}} & =1-1+\frac{\sqrt{x}}{\sqrt{x+\sqrt{x}}}=1-\frac{\sqrt{x+\sqrt{x}}-\sqrt{x}}{\sqrt{x+\sqrt{x}}}=1-\frac{x+\sqrt{x}-x}{\sqrt{x+\sqrt{x}}(\sqrt{x+\sqrt{x}}+\sqrt{x})} \\ & =1-\frac{\sqrt{x}}{x+\sqrt{x}+x \cdot \sqrt{1+\frac{1}{\sqrt{x}}}}=1-\frac{1}{1+\sqrt{x} \cdot\left(1+\sqrt{1+\frac{1}{\sqrt{x}}}\right)} .\end{aligned}$
